More cleanup

src/new_goose_lang/lib/struct/struct.v
@@ -4,8 +4,29 @@ From Perennial.goose_lang Require Import proofmode.
 From Perennial.new_goose_lang.lib Require Export typed_mem struct.impl.
 From Perennial.Helpers Require Import NamedProps.
 
-Local Close Scope struct_scope.
+Notation "l ↦s[ d :: f ] dq v" := (struct.fieldRef_f d f l ↦[struct.fieldTy d f]{dq} v)%I
+  (at level 50, dq custom dfrac at level 70, d at level 59, f at level 59,
+     format "l  ↦s[ d :: f ] dq  v").
 
-Reserved Notation "l ↦[ d :: f ] dq v"
-    (at level 20, dq custom dfrac at level 1, d at level 50, f at level 50,
-       format "l  ↦[ d :: f ] dq  v").
+Section lemmas.
+Context `{heapGS Σ}.
+(* FIXME: move this *)
+Local Fixpoint struct_big_fields_rec l dq (d: descriptor) (fs:descriptor) (v:val): iProp Σ :=
+  match fs with
+  | [] => "_" ∷ ⌜v = #()⌝
+  | (f,t)::fs =>
+    match v with
+    | PairV v1 v2 => ("H" ++ f) ∷ l ↦s[d :: f]{dq} v1 ∗
+                    struct_big_fields_rec l dq d fs v2
+    | _ => False
+    end
+  end.
+
+Definition struct_fields l dq d v : iProp Σ := struct_big_fields_rec l dq d d v.
+
+Theorem struct_fields_split l q d {dwf: struct.wf d} v :
+  typed_pointsto l q (structT d) v ⊣⊢ struct_fields l q d v.
+Proof.
+Admitted.
+
+End lemmas.
