src/new_goose_lang/lib/slice/impl.v
@@ -1,5 +1,4 @@
 From Perennial.goose_lang Require Import notation.
-From Perennial.new_goose_lang Require Import typing.
 From Perennial.new_goose_lang.lib Require Import typed_mem.impl.
 From Perennial.goose_lang.lib Require Import control.impl.
 
