src/new_goose_lang/lib/slice/slice.v
@@ -1,7 +1,6 @@
 From RecordUpdate Require Import RecordSet.
 From Perennial.Helpers Require Import List Fractional.
 From Perennial.goose_lang Require Import proofmode.
-(* From Perennial.new_goose_lang.lib Require Import persistent_readonly typed_mem. *)
 From Perennial.new_goose_lang.lib Require Export slice.impl.
 From Perennial.goose_lang.lib Require Import control.control.
 
