src/new_goose_lang/prelude.v
@@ -1,5 +1,5 @@
 From Perennial.goose_lang Require Export lang notation.
-From Perennial.new_goose_lang Require Export exception loop.impl struct.impl typed_mem.impl typing.
+From Perennial.new_goose_lang Require Export exception loop.impl struct.impl typed_mem.impl.
 From Perennial.goose_lang.lib Require Export
      encoding.impl map.impl slice.impl
      time.impl rand.impl string.impl channel.impl
